

Emmanuel Gomez
135:

d) 90-

$$1) a - x^2 = 2x + 3$$

$$\Leftrightarrow 2x + 3 - x^2 = 0$$

$$\Delta = b^2 - 4ac$$

$$= 2^2 - 4 \times (-1) \times 3$$

$$= 16 > 0 \quad \text{donc 2 racines}$$

$$x_1 = \frac{-b + \sqrt{\Delta}}{2a}$$

$$= \frac{-2 + \sqrt{16}}{-1 \times 2}$$

$$= -1$$

$$y_1 = 2 \times (-1) + 3$$

$$= 1$$

$$A(-1; 1)$$

$$x_2 = \frac{-b - \sqrt{\Delta}}{2a}$$

$$= \frac{-2 - \sqrt{16}}{-1 \times 2}$$

$$= 3$$

$$y_2 = 2 \times 3 + 3$$

$$= 9$$

$$B(3; 9)$$

$$5) H\left(\frac{-1+3}{2}, \frac{1+9}{2}\right)$$

$$H(1; 5)$$

$$2) \frac{y_B - y_A}{x_B - x_A} = \frac{9 - 1}{3 - (-1)} = \frac{8}{4} = 2$$

Le coefficient directeur de la droite (AB) est de 2.

$$b) (x^2)' = 2x$$

$$(2x + 3)' = 2$$

$$2x = 2$$

$$x = \frac{2}{2} = 1$$

donc l'abscisse de C est 1 donc C et H ont la même abscisse.